# Own prefixes
@base             <http://data.tbfy.eu/> .
@prefix tbfy:     <http://data.tbfy.eu/ontology/tbfy/> . 
@prefix ocds:     <http://data.tbfy.eu/ontology/ocds/> .
@prefix ebg:      <http://data.businessgraph.io/ontology#/> .

# External prefixes
@prefix dc:       <http://purl.org/dc/terms/> .
@prefix foaf:     <http://xmlns.com/foaf/0.1/> .
@prefix owl:      <http://www.w3.org/2002/07/owl#> .
@prefix rdf:      <http://www.w3.org/1999/02/22-rdf-syntax-ns#> .
@prefix schema:   <http://schema.org/> .
@prefix xsd:      <http://www.w3.org/2004/02/skos/core#> .

# Imports
<http://data.tbfy.eu/ontology/tbfy> rdf:type owl:Ontology ;
  owl:imports <http://data.tbfy.eu/ontology/ocds/> , <http://data.businessgraph.io/ontology#/> .


# Ontology
tbfy:companyReconciliationScore a owl:DatatypeProperty ;
  schema:domainIncludes ocds:Organisation ;
  schema:rangeIncludes xsd:integer ;
  rdfs:label "matching score" ;
  skos:definition "Score value from the Reconciliation API." ;
  skos:scopeNote "Only applicable to matching suppliers for which there exist a sameAs link." . 

tbfy:companyReconciliationSource a owl:DatatypeProperty ;
  schema:domainIncludes ocds:Organisation ;
  schema:rangeIncludes xsd:string ;
  rdfs:label "matching source" ;
  skos:definition "Source of the matching, i.e., the URL to the Reconciliation API or an URI to a person (crowdsourcing)." ;
  skos:scopeNote "Only applicable to matching suppliers for which there exist a sameAs link." . 
